forward.v is compiled, but forward tactic still has problem

CSplit/strong.v
@@ -2871,3 +2871,200 @@ split;intro.
   try (intros; solve_andp).
   auto.
 Qed.
+
+
+Theorem seq_assoc:
+  forall {CS: compspecs} {Espec: OracleKind},
+   forall Delta P s1 s2 s3 R,
+        @semax CS Espec Delta P (Ssequence s1 (Ssequence s2 s3)) R <->
+        @semax CS Espec Delta P (Ssequence (Ssequence s1 s2) s3) R.
+Proof.
+  intros.
+  split; intros.
+  + apply semax_seq_inv in H.
+    destruct H as [? [? ?]].
+    apply semax_seq_inv in H0.
+    destruct H0 as [? [? ?]].
+    eapply semax_seq; eauto.
+    eapply semax_seq; eauto.
+    destruct R; auto.
+  + apply semax_seq_inv in H.
+    destruct H as [? [? ?]].
+    apply semax_seq_inv in H.
+    destruct H as [? [? ?]].
+    eapply semax_seq with x0; [destruct R; exact H |].
+    eapply semax_seq; eauto.
+Qed.
+
+
+Lemma semax_if_seq:
+ forall {CS: compspecs} {Espec: OracleKind} Delta P e c1 c2 c Q,
+ semax Delta P (Sifthenelse e (Ssequence c1 c) (Ssequence c2 c)) Q ->
+ semax Delta P (Ssequence (Sifthenelse e c1 c2) c) Q.
+Proof.
+  intros.
+  apply semax_ifthenelse_inv in H.
+  eapply semax_conseq; [exact H | intros; apply derives_aux_refl .. |].
+  rewrite exp_andp2.
+  apply semax_extract_exists.
+  intros P'.
+  rewrite andp_comm, andp_assoc.
+  apply semax_extract_prop; intros [? ?].
+  rewrite andp_comm.
+  apply semax_seq_inv in H0.
+  apply semax_seq_inv in H1.
+  destruct H0 as [Q1 [? ?]], H1 as [Q2 [? ?]].
+  apply semax_seq with (orp Q1 Q2); [apply semax_ifthenelse |].
+  + eapply semax_post; [| | | | exact H0].
+    - destruct Q; apply andp_left2, orp_right1, derives_refl.
+    - destruct Q; apply andp_left2, derives_refl.
+    - destruct Q; apply andp_left2, derives_refl.
+    - intro; destruct Q; apply andp_left2, derives_refl.
+  + eapply semax_post; [| | | | exact H1].
+    - destruct Q; apply andp_left2, orp_right2, derives_refl.
+    - destruct Q; apply andp_left2, derives_refl.
+    - destruct Q; apply andp_left2, derives_refl.
+    - intro; destruct Q; apply andp_left2, derives_refl.
+  + rewrite orp_is_exp.
+    apply semax_extract_exists.
+    intro.
+    destruct x; auto.
+Qed.
+
+
+Definition semax_equiv {CS: compspecs} {Espec: OracleKind} c1 c2: Prop := forall Delta P Q, semax Delta P c1 Q <-> semax Delta P c2 Q.
+
+Lemma semax_equiv_seq: forall {CS: compspecs} {Espec: OracleKind} c1 c2 c3 c4,
+  semax_equiv c1 c2 ->
+  semax_equiv c3 c4 ->
+  semax_equiv (Ssequence c1 c3) (Ssequence c2 c4).
+Proof.
+  intros.
+  hnf; intros; split; intros.
+  + apply semax_seq_inv in H1.
+    destruct H1 as [? [? ?]].
+    rewrite (H Delta P _) in H1.
+    rewrite (H0 Delta _ _) in H2.
+    eapply semax_seq; eauto.
+  + apply semax_seq_inv in H1.
+    destruct H1 as [? [? ?]].
+    rewrite <- (H Delta P _) in H1.
+    rewrite <- (H0 Delta _ _) in H2.
+    eapply semax_seq; eauto.
+Qed.
+
+Lemma semax_equiv_sym: forall {CS: compspecs} {Espec: OracleKind} c1 c2, semax_equiv c1 c2 -> semax_equiv c2 c1.
+Proof.
+  intros.
+  hnf in H |- *.
+  intros.
+  specialize (H Delta P Q).
+  tauto.
+Qed.
+
+Lemma semax_equiv_trans: forall {CS: compspecs} {Espec: OracleKind} c1 c2 c3, semax_equiv c1 c2 -> semax_equiv c2 c3 -> semax_equiv c1 c3.
+Proof.
+  intros.
+  hnf in H, H0 |- *.
+  intros.
+  specialize (H Delta P Q).
+  specialize (H0 Delta P Q).
+  tauto.
+Qed.
+
+
+Fixpoint fold_Ssequence lc :=
+  match lc with
+  | nil => Sskip
+  | c1 :: nil => c1
+  | c :: lc0 => Ssequence c (fold_Ssequence lc0)
+  end.
+
+
+Definition non_Sseq c :=
+  match c with
+  | Ssequence _ _ => False
+  | _ => True
+  end.
+
+Inductive unfold_Sseq_rel: statement -> list statement -> Prop :=
+  | singleton: forall c, non_Sseq c -> unfold_Sseq_rel c (c :: nil)
+  | tl_step: forall c1 c2 lc, non_Sseq c1 -> unfold_Sseq_rel c2 lc ->
+                 unfold_Sseq_rel (Ssequence c1 c2) (c1 :: lc)
+  | hd_step: forall c1 c2 c3 lc, unfold_Sseq_rel (Ssequence c1 (Ssequence c2 c3)) lc ->
+                 unfold_Sseq_rel (Ssequence (Ssequence c1 c2) c3) lc
+  .
+
+Lemma unfold_Sseq_rel_non_nil: forall {c} {P: Prop}, unfold_Sseq_rel c nil -> P.
+Proof.
+  intros.
+  remember nil as lc.
+  induction H.
+  + congruence.
+  + congruence.
+  + auto.
+Qed.
+
+Lemma unfold_Sseq_rel_sound: forall {CS: compspecs} {Espec: OracleKind} c lc,
+  unfold_Sseq_rel c lc -> semax_equiv (fold_Ssequence lc) c.
+Proof.
+  intros.
+  induction H.
+  + simpl.
+    hnf; intros; tauto.
+  + simpl.
+    destruct lc; [apply (unfold_Sseq_rel_non_nil H0) |].
+    apply semax_equiv_seq; [hnf; intros; tauto | assumption].
+  + eapply semax_equiv_trans; [eauto |].
+    hnf; intros.
+    apply seq_assoc.
+Qed.
+
+Lemma unfold_Ssequence_unfold_Sseq_rel: forall c, unfold_Sseq_rel c (unfold_Ssequence c).
+Proof.
+  intros.
+  induction c; try solve [apply singleton, I].
+  revert c2 IHc2.
+  clear IHc1.
+  induction c1; intros; try solve [apply tl_step; [apply I | auto]].
+  apply hd_step.
+  replace (unfold_Ssequence (Ssequence (Ssequence c1_1 c1_2) c2)) with
+    (unfold_Ssequence (Ssequence c1_1 (Ssequence c1_2 c2))).
+  2:{
+    simpl.
+    rewrite <- app_assoc.
+    reflexivity.
+  }
+  apply IHc1_1.
+  apply IHc1_2.
+  apply IHc2.
+Qed.
+
+Lemma unfold_Ssequence_sound: forall {CS: compspecs} {Espec: OracleKind} c, semax_equiv (fold_Ssequence (unfold_Ssequence c)) c.
+Proof.
+  intros.
+  apply unfold_Sseq_rel_sound.
+  apply unfold_Ssequence_unfold_Sseq_rel.
+Qed.
+
+Lemma semax_unfold_Ssequence': forall {CS: compspecs} {Espec: OracleKind} c1 c2,
+  unfold_Ssequence c1 = unfold_Ssequence c2 ->
+  (forall P Q Delta, semax Delta P c1 Q <-> semax Delta P c2 Q).
+Proof.
+  intros.
+  eapply semax_equiv_trans.
+  + apply semax_equiv_sym.
+    apply unfold_Ssequence_sound.
+  + rewrite H.
+    apply unfold_Ssequence_sound.
+Qed.
+
+Lemma semax_unfold_Ssequence: forall {CS: compspecs} {Espec: OracleKind} c1 c2,
+  unfold_Ssequence c1 = unfold_Ssequence c2 ->
+  (forall P Q Delta, @semax CS Espec Delta P c1 Q -> @semax CS Espec Delta P c2 Q).
+Proof.
+  intros.
+  pose proof semax_unfold_Ssequence' _ _ H.
+  clear - H0 H1.
+  firstorder.
+Qed.
