floyd-seq/forward.v
@@ -30,6 +30,7 @@ Require Import FloydSeq.diagnosis.
 Require Import FloydSeq.simpl_reptype.
 Require Import FloydSeq.nested_pred_lemmas.
 Require Import FloydSeq.freezer.
+Require Import CSplit.strong.
 Import Cop.
 Import Cop2.
 Import Clight_Cop2.
@@ -283,7 +284,8 @@ Ltac semax_func_skipn :=
 Ltac LookupID := first [ cbv;reflexivity | fail "Lookup for a function identifier in Genv failed" ].
 Ltac LookupB := first [ cbv;reflexivity | fail "Lookup for a function pointer block in Genv failed" ].
 
-Lemma semax_body_subsumption' cs cs' V V' F F' f spec
+(* [litao] semaxbody removed *)
+(* Lemma semax_body_subsumption' cs cs' V V' F F' f spec
       (SF: @semax_body V F cs f spec)
       (CSUB: cspecs_sub cs cs')
       (COMPLETE : Forall (fun it : ident * type => complete_type (@cenv_cs cs) (snd it) = true) (fn_vars f))
@@ -293,7 +295,7 @@ Proof.
   intros.
   apply (@semax_body_cenv_sub _ _ CSUB); auto.
   eapply semax_body_subsumption; try eassumption.
-Qed.
+Qed. *)
 
 Lemma sub_option_get' {A: Type} (s t: PTree.t A) B (f:A -> option B):
   Forall (fun x => PTree.get (fst x) t = Some (snd x)) (PTree.elements s) ->
@@ -435,7 +437,7 @@ eapply (@semax_body_subsumption' _ _ _ _ _ _ _ _ L);
  | simple apply tycontext_sub_refl ||
   (apply tycontext_sub_i99; assumption)].
 *)
-Ltac apply_semax_body L := 
+(* Ltac apply_semax_body L := 
 eapply (@semax_body_subsumption' _ _ _ _ _ _ _ _ L);
   [ first [ apply cspecs_sub_refl
           | split3; red; apply @sub_option_get; 
@@ -476,7 +478,7 @@ Ltac semax_func_cons L :=
              ]
         ];
  repeat (eapply semax_func_cons_ext_vacuous; [reflexivity | reflexivity | LookupID | LookupB |]);
- try apply semax_func_nil.
+ try apply semax_func_nil. *)
 
 (* This is a better way of finding an element in a long list. *)
 Lemma from_elements_In : forall {A} l i (v : A), (pTree_from_elements l) ! i = Some v ->
@@ -506,7 +508,7 @@ intros.
  apply prop_right; auto.
 Qed.
 
-Ltac semax_func_cons_ext :=
+(* Ltac semax_func_cons_ext :=
  repeat (eapply semax_func_cons_ext_vacuous; [reflexivity | reflexivity | LookupID | LookupB | ]);
   eapply semax_func_cons_ext;
     [ reflexivity | reflexivity | reflexivity | reflexivity | reflexivity
@@ -524,7 +526,7 @@ Ltac semax_func_cons_ext :=
               "Make sure that the Espec declared using 'Existing Instance'
                is defined as 'add_funspecs NullExtension.Espec Gprog.'"
     |
-    ].
+    ]. *)
 
 Tactic Notation "forward_seq" :=
   first [eapply semax_seq'; [  | abbreviate_semax ]
@@ -1325,6 +1327,7 @@ Ltac prove_call_setup ts subsumes witness :=
  end;
  prove_call_setup_aux ts witness].
 
+
 Ltac fwd_call' ts subsumes witness :=
 lazymatch goal with
 | |- semax _ _ (Ssequence (Scall _ _ _) _) _ =>
@@ -2065,7 +2068,7 @@ Proof.
 intros. apply pred_ext. Exists tt. auto. Intros u; auto.
 Qed.
 
-Tactic Notation "forward_while" constr(Inv) :=
+(* Tactic Notation "forward_while" constr(Inv) :=
   repeat (apply -> seq_assoc; abbreviate_semax);
   lazymatch goal with |- semax _ _ (Ssequence _ _) _ => idtac | _ => apply <- semax_seq_skip end;
   first [ignore (Inv: environ->mpred)
@@ -2135,7 +2138,7 @@ Loop test expression:" e
          normalize in HRE
        ]
     ]; abbreviate_semax; 
-    simpl_ret_assert (*autorewrite with ret_assert*).
+    simpl_ret_assert (*autorewrite with ret_assert*). *)
 
 
 Inductive Type_of_invariant_in_forward_for_should_be_environ_arrow_mpred_but_is : Type -> Prop := .
@@ -2152,7 +2155,7 @@ Ltac check_type_forward_for_simple_bound :=
          end
      end.
 
-Ltac forward_for_simple_bound n Pre :=
+(* Ltac forward_for_simple_bound n Pre :=
   check_Delta; check_POSTCONDITION;
  repeat match goal with |-
       semax _ _ (Ssequence (Ssequence (Ssequence _ _) _) _) _ =>
@@ -2214,7 +2217,7 @@ Ltac forward_for3 Inv PreInc Postcond :=
             end ]
        | abbreviate_semax;
          repeat (apply semax_extract_PROP; fancy_intro true)
-      ].
+      ]. *)
 
 Fixpoint no_breaks (s: statement) : bool :=
  match s with
@@ -2225,7 +2228,7 @@ Fixpoint no_breaks (s: statement) : bool :=
  | _ => true
  end.
 
-Ltac forward_for2 Inv PreInc :=
+(* Ltac forward_for2 Inv PreInc :=
  repeat  match goal with P := @abbreviate ret_assert _ |- semax _ _ _ ?P' =>
                          constr_eq P P'; unfold abbreviate in P; subst P
            end;
@@ -2250,14 +2253,16 @@ Ltac forward_for2 Inv PreInc :=
             repeat (apply semax_extract_PROP; fancy_intro true);
             do_repr_inj HRE
         ]    
-  end.
+  end. *)
 
 Lemma seq_assoc1: 
    forall (Espec: OracleKind) (CS : compspecs) (Delta : tycontext) (P : environ -> mpred)
          (s1 s2 s3 : statement) (R : ret_assert),
        semax Delta P (Ssequence s1 (Ssequence s2 s3)) R ->
        semax Delta P (Ssequence (Ssequence s1 s2) s3) R.
-Proof. intros. apply -> seq_assoc; auto. Qed.
+Proof. intros. 
+apply -> seq_assoc; auto. Qed.
+
 
 Lemma semax_loop_noincr :
   forall {Espec: OracleKind}{CS: compspecs} ,
@@ -2411,19 +2416,19 @@ Ltac check_nocontinue s :=
  | _ => fail 100 "applied forward_loop to something that is not a loop"
 end.
 
-Ltac forward_loop_nocontinue2 Inv :=
-  apply semax_loop_nocontinue; delete_skip; abbreviate_semax.
+(* Ltac forward_loop_nocontinue2 Inv :=
+  apply semax_loop_nocontinue; delete_skip; abbreviate_semax. *)
 
-Ltac forward_loop_nocontinue1 Inv :=
+(* Ltac forward_loop_nocontinue1 Inv :=
   lazymatch goal with
   | |- semax _ _ (Sfor _ _ _ _) _ => apply semax_seq' with Inv; [abbreviate_semax | forward_loop_nocontinue2 Inv]
   | |- semax _ _ (Sloop _ _) _ => apply semax_pre with Inv; [ | forward_loop_nocontinue2 Inv]
   | |- semax _ _ (Swhile ?E ?B) _ => 
           let x := fresh "x" in set (x := Swhile E B); unfold Swhile at 1 in x; subst x;
           apply semax_pre with Inv; [ | forward_loop_nocontinue2 Inv]
- end.
+ end. *)
 
-Ltac forward_loop_nocontinue Inv Post :=
+(* Ltac forward_loop_nocontinue Inv Post :=
   repeat simple apply seq_assoc1;
   repeat apply -> semax_seq_skip;
   match goal with
@@ -2432,9 +2437,9 @@ Ltac forward_loop_nocontinue Inv Post :=
   | |- semax _ _ _ ?Post' => 
             tryif (unify Post Post') then forward_loop_nocontinue1 Inv
            else (apply (semax_post1_flipped Post); [ forward_loop_nocontinue1 Inv  | ])
-  end.
+  end. *)
 
-Ltac forward_loop_nocontinue_nobreak Inv :=
+(* Ltac forward_loop_nocontinue_nobreak Inv :=
  repeat apply -> semax_seq_skip;
   lazymatch goal with
   | |- semax _ _ (Ssequence (Swhile _ ?S) _) _ =>
@@ -2450,9 +2455,9 @@ Ltac forward_loop_nocontinue_nobreak Inv :=
      forward_loop_nocontinue Inv Post
   | |- semax _ _ _ _ => fail 100 "forward_loop failed; try doing abbreviate_semax first"
   | |- _ => fail 100 "forward_loop applicable only to a semax goal"
-end.
+end. *)
 
-Tactic Notation "forward_loop" constr(Inv)  := 
+(* Tactic Notation "forward_loop" constr(Inv)  := 
  repeat simple apply seq_assoc1;
  repeat apply -> semax_seq_skip;
   lazymatch goal with
@@ -2465,9 +2470,9 @@ Tactic Notation "forward_loop" constr(Inv)  :=
   tryif (check_nocontinue c)
    then forward_loop_nocontinue_nobreak Inv
   else (check_no_incr c; forward_loop Inv continue: Inv)
- end.
+ end. *)
 
-Tactic Notation "forward_loop" constr(Inv) "break:" constr(Post) :=
+(* Tactic Notation "forward_loop" constr(Inv) "break:" constr(Post) :=
  repeat simple apply seq_assoc1;
  repeat apply -> semax_seq_skip;
   lazymatch goal with
@@ -2480,9 +2485,9 @@ Tactic Notation "forward_loop" constr(Inv) "break:" constr(Post) :=
   tryif (check_nocontinue c)
    then forward_loop_nocontinue Inv Post
   else (check_no_incr c; forward_loop Inv continue: Inv break: Post)
- end.
+ end. *)
 
-Tactic Notation "forward_for" constr(Inv) "continue:" constr(PreInc) :=
+(* Tactic Notation "forward_for" constr(Inv) "continue:" constr(PreInc) :=
   check_Delta; check_POSTCONDITION;
   repeat simple apply seq_assoc1;
   lazymatch type of Inv with
@@ -2516,9 +2521,9 @@ Tactic Notation "forward_for" constr(Inv) "continue:" constr(PreInc) :=
      apply semax_pre with (exp Inv);
       [ unfold_function_derives_right | forward_for2 Inv PreInc ]
   | |- _ => fail "forward_for2x cannot recognize the loop"
-  end.
+  end. *)
 
-Tactic Notation "forward_for" constr(Inv) "continue:" constr(PreInc) "break:" constr(Postcond) :=
+(* Tactic Notation "forward_for" constr(Inv) "continue:" constr(PreInc) "break:" constr(Postcond) :=
   check_Delta; check_POSTCONDITION;
   repeat simple apply seq_assoc1;
   lazymatch type of Inv with
@@ -2541,10 +2546,10 @@ Tactic Notation "forward_for" constr(Inv) "continue:" constr(PreInc) "break:" co
   | |- semax _ _ (Sloop (Ssequence (Sifthenelse _ Sskip Sbreak) _) _) _ =>
      apply semax_pre with (exp Inv);
       [ unfold_function_derives_right | forward_for3 Inv PreInc Postcond ]
-  end.
+  end. *)
 
-Tactic Notation "forward_for" constr(Inv) "break:" constr(Postcond) "continue:" constr(PreInc) :=
-   forward_for Inv continue: PreInc break: Postcond.
+(* Tactic Notation "forward_for" constr(Inv) "break:" constr(Postcond) "continue:" constr(PreInc) :=
+   forward_for Inv continue: PreInc break: Postcond. *)
 
 Tactic Notation "forward_for" constr(Inv) constr(PreInc) :=
   fail "Usage of the forward_for tactic:
@@ -2552,7 +2557,7 @@ forward_for  Inv   (* where Inv: A->environ->mpred is a predicate on index value
 forward_for Inv continue: PreInc (* where Inv,PreInc are predicates on index values of type A *)
 forward_for Inv continue: PreInc break:Post (* where Post: environ->mpred is an assertion *)".
 
-Lemma semax_convert_for_while:
+(* Lemma semax_convert_for_while:
  forall CS Espec Delta Pre s1 e2 s3 s4 Post,
   nocontinue s4 = true ->
   nocontinue s3 = true ->
@@ -2566,9 +2571,9 @@ apply -> semax_seq_skip in H1; auto.
 apply seq_assoc in H1; auto.
 apply <- semax_seq_skip.
 apply H2; auto.
-Qed.
+Qed. *)
 
-Tactic Notation "forward_for" constr(Inv) :=
+(* Tactic Notation "forward_for" constr(Inv) :=
   check_Delta; check_POSTCONDITION;
   repeat simple apply seq_assoc1;
   lazymatch type of Inv with
@@ -2592,7 +2597,7 @@ Tactic Notation "forward_for" constr(Inv) :=
                    [  |  forward_while (EX x:_, Inv x);
                              [ apply ENTAIL_refl | | | eapply semax_post_flipped'; [apply semax_skip | ] ]  ] ]
         
-  end.
+  end. *)
 
 Ltac process_cases sign := 
 match goal with
@@ -2632,7 +2637,7 @@ match goal with
 end.
 
 
-Ltac forward_switch' := 
+(* Ltac forward_switch' := 
 match goal with
 | |- semax ?Delta (PROPx ?P (LOCALx ?Q (SEPx ?R))) (Sswitch ?e _) _ =>
    let sign := constr:(signof e) in let sign := eval hnf in sign in
@@ -2657,7 +2662,7 @@ match goal with
              try match goal with H := @abbreviate statement _ |- _ => clear H end;
              process_cases sign ]
 ]
-end.
+end. *)
 
 
 Definition nofallthrough ek :=
@@ -2698,7 +2703,8 @@ match goal with
 | |- semax _ (@exp _ _ _ _) _ _ =>
       fail "First use Intros ... to take care of the EXistentially quantified variables in the precondition"
 | |- semax _ _ (Sswitch _ _) _ =>
-  forward_switch'
+  (* forward_switch' *)
+  fail "no support in VST-A"
 | |- semax _ _ (Ssequence (Sifthenelse _ _ _) _) _ => 
      fail "forward_if failed for some unknown reason, perhaps your precondition is not in canonical form"
 | |- semax _ _ (Ssequence (Sswitch _ _) _) _ => 
@@ -2738,7 +2744,9 @@ match goal with
  | |- semax _ _ (Sifthenelse _ _ _) (overridePost post _) =>
        forward_if'_new
  | |- semax _ _ (Sswitch _ _) _ =>
-       forward_switch'
+       (* forward_switch' *)
+
+       fail "not support switch in VST-A"
  | |- semax _ _ (Sifthenelse _ _ _) ?P =>
       apply (semax_post_flipped (overridePost post P));
       [ forward_if'_new
@@ -2760,10 +2768,11 @@ match goal with
       | abbreviate_semax; 
         simpl_ret_assert (*autorewrite with ret_assert*)]
    | |- semax _ _ (Ssequence (Sswitch _ _) _) _ =>
-     apply semax_seq with post;
+     (* apply semax_seq with post;
       [forward_switch' 
       | abbreviate_semax; 
-        simpl_ret_assert (*autorewrite with ret_assert*)]
+        simpl_ret_assert (*autorewrite with ret_assert*)] *)
+        fail "not support switch in VST-A"
 end.
 
 Ltac remove_LOCAL name Q :=
@@ -4158,7 +4167,7 @@ split; simpl.
 Qed.
 
 
-Ltac start_function :=
+(* Ltac start_function :=
  leaf_function;
  match goal with |- semax_body ?V ?G ?F ?spec =>
     check_normalized F;
@@ -4251,7 +4260,7 @@ Ltac start_function :=
  try match goal with DS := @abbreviate (PTree.t funspec) PTree.Leaf |- _ =>
      clearbody DS
  end;
- start_function_hint.
+ start_function_hint. *)
 
 Opaque sepcon.
 Opaque emp.
@@ -4502,9 +4511,9 @@ Ltac with_library' p G :=
 Ltac with_library prog G :=
   let pr := eval unfold prog in prog in  with_library' pr G.
 
-Definition semax_prog {Espec} {CS} prog z V G :=
+(* Definition semax_prog {Espec} {CS} prog z V G :=
  @SeparationLogicAsLogicSoundness.MainTheorem.CSHL_MinimumLogic.CSHL_Defs.semax_prog
-  Espec CS prog z V (augment_funspecs prog G).
+  Espec CS prog z V (augment_funspecs prog G). *)
 
 Lemma mk_funspec_congr:
   forall a b c d e f g a' b' c' d' e' f' g',
@@ -4519,7 +4528,7 @@ subst d' e'.
 f_equal; apply proof_irr.
 Qed.
 
-Ltac prove_semax_prog_old :=
+(* Ltac prove_semax_prog_old :=
  split3; [ | | split3; [ | | split]];
  [ reflexivity || fail "duplicate identifier in prog_defs"
  | reflexivity || fail "unaligned initializer"
@@ -4536,7 +4545,7 @@ Ltac prove_semax_prog_old :=
         fail "Funspec of _main is not in the proper form"
     end
  ];
- repeat (eapply semax_func_cons_ext_vacuous; [reflexivity | reflexivity | reflexivity | LookupID | LookupB | ]).
+ repeat (eapply semax_func_cons_ext_vacuous; [reflexivity | reflexivity | reflexivity | LookupID | LookupB | ]). *)
 
 (**************MATERIAL FOR NEW TACTIC prove_semax_prog STARTS HERE ***************)
 
@@ -4663,7 +4672,7 @@ Ltac solve_cenvcs_goal :=
   solve [repeat f_equal; finish_composites])
  || (cbv; repeat f_equal; apply proof_irr).
 
-Ltac prove_semax_prog_aux tac :=
+(* Ltac prove_semax_prog_aux tac :=
   match goal with
     | |- semax_prog ?prog ?z ?Vprog ?Gprog =>
      let x := constr:(ltac:(old_with_library prog Gprog))
@@ -4689,11 +4698,11 @@ Ltac prove_semax_prog_aux tac :=
    pose (Gprog := @abbreviate _ G); 
   change (semax_func V Gprog g D G')
  end;
- tac.
+ tac. *)
 
-Ltac finish_semax_prog := repeat (eapply semax_func_cons_ext_vacuous; [reflexivity | reflexivity | LookupID | LookupB | ]).
+(* Ltac finish_semax_prog := repeat (eapply semax_func_cons_ext_vacuous; [reflexivity | reflexivity | LookupID | LookupB | ]). *)
 
-Ltac prove_semax_prog := prove_semax_prog_aux finish_semax_prog.
+(* Ltac prove_semax_prog := prove_semax_prog_aux finish_semax_prog. *)
 
 (*******************************************)
 
